
\documentclass[11pt]{article}

\input{../../tex/defs.tex}

% Useful syntax commands
\newcommand{\jarr}[1]{\left[#1\right]}   % \jarr{x: y} = {x: y}
\newcommand{\jobj}[1]{\left\{#1\right\}} % \jobj{1, 2} = [1, 2]
\newcommand{\pgt}[1]{\, > {#1}}          % \pgt{1} = > 1
\newcommand{\plt}[1]{\, < {#1}}          % \plt{2} = < 2
\newcommand{\peq}[1]{\, = {#1}}          % \peq{3} = = 3
\newcommand{\prop}[1]{\langle{#1}\rangle}% \prop{x} = <x>
\newcommand{\matches}[2]{{#1}\sim{#2}}   % \matches{a}{b} = a ~ b
\newcommand{\aeps}{\varepsilon}          % \apes = epsilon
\newcommand{\akey}[2]{.{#1}\,{#2}}       % \akey{s}{a} = .s a
\newcommand{\aidx}[2]{[#1]\,{#2}}        % \aidx{i}{a} = [i] a
\newcommand{\apipe}[1]{\mid {#1}}        % \apipe{a} = | a

% Other useful syntax commands:
%
% \msf{x} = x (not italicised)
% \falset = false
% \truet = true
% \tnum = num
% \tbool = bool
% \tstr = str


\begin{document}

\hwtitle
  {Assignment 1}
  {Vivek Pandya (vpandya)} %% REPLACE THIS WITH YOUR NAME/ID

\problem{Problem 1}

Part 1:

\begin{alignat*}{1}
\msf{NumerOperation}~nop ::= \qamp = \mid \ne \mid < \mid > \\
\msf{StringOperation}~sop ::= \qamp = \mid \ne \\ 
\msf{Property}~p ::= \qamp \varepsilon \\
\mid \qamp nop \, \msf{n} \\
\mid \qamp sop \, \msf{s} \\
\mid \qamp \msf{p1} \vee \msf{p2} \\
\mid \qamp \msf{p1} \wedge \msf{p2} \\
\\
\msf{bool} ::= \qamp true \mid false \\
\msf{Schema}~\tau ::= \qamp \tnum \prop{p} \\
\mid \qamp \tstr \prop{p}\\
\mid \qamp \msf{bool} \\
\mid \qamp [\, \tau ]\, \\
\mid \qamp \{ (\, s : \tau)\, ^{*}\} \\
\end{alignat*}

Part 2:

% mathpar is the environment for writing inference rules. It takes care of
% the spacing and line breaks automatically. Use "\\" in the premises to
% space out multiple assumptions.
\begin{mathpar}

\ir{S-Bool-False}{\ }{\matches{\falset}{\tbool}}

\ir{S-Bool-True}{\ }{\matches{\truet}{\tbool}}
\\
\ir{S-Num}{\ }{\matches{n}{\tnum}} 

\ir{S-String}{\ }{\matches{s}{\tstr}}

\\

\ir{S-Num-Property}{(n \, nop\, n_{1})}{\matches{n}{(\tnum<nop\, n_{1}>)}}

\ir{S-String-Property}{(s \, sop\, s_{1})}{\ \matches{s}{\tstr<sop \, s_{1}>} }
%\ir{S-Number1}{\ ( n > 0  \thinspace \wedge n < 5 ) }{\matches{n}{\tau}}

%\ir{S-Number2}{\ n = 10 }{\matches{n}{\tau}}

\\
\ir{S-Num-Property-And}{\matches{n}{\tnum<p1>} \,\,\,\,\, \matches{n}{\tnum<p2>}}{\matches{n}{\tnum<p_1 \wedge p_2>}}

\ir{S-Num-Property-Or}{\matches{n}{\tnum<p_1>}}{\matches{n}{\tnum<p_1 \vee p_2>}}

\ir{S-String-Property-And}{\matches{s}{\tstr<p1>} \,\,\,\,\, \matches{s}{\tstr<p2>}}{\matches{s}{\tstr<p_1 \wedge p_2>}}

\ir{S-String-Property-Or}{\matches{s}{\tstr<p_1>}}{\matches{s}{\tstr<p_1 \vee p_2>}}

\\
\ir{S-Empty-Object}{\ }{\matches{\{ \}}{\tau}}

\ir{S-Empty-Array}{\ }{\matches{[ \, ] \,}{\tau}}

\\

%\ir{S-Obj1}{\matches{K_1}{\tstr} \; \matches{V_1}{\tbool}  \; \matches{K_2}{\tstr} \; V_2 = X  }{ \matches{\{ K_1 : V_1, K_2 : V_2\}}{\tau}}

%\ir{S-Obj2}{\matches{K_1}{\tstr} \; \matches{V_1}{\tbool}  \; \matches{K_2}{\tstr} \; V_2 = Y  }{ \matches{\{ K_1 : V_1, K_2 : V_2\}}{\tau}}
\\


\ir{S-Array}{ \forall i \in [|j|]. \matches{j_{i}}{\tau} }{\matches{ [\, j_1, ..., j_n]\,}{\tau} }

\ir{S-Object}{\ \forall s^{'} \in s. \matches{j_{s^{'}}}{\tau} }{\matches{\{ (s : j)^{*} \}}{\tau} }

%\ir{S-Array-Element-0}{\matches{K}{\tstr} \; V = 0 }{\matches{[ \, \{ K : V \} ] \, }{\msf{\tau}}}

%\ir{S-Array-Step1}{\matches{K_0}{\tstr} \;  \matches{V_0}{\tnum}  \; \matches{K_1}{\tstr} \; \matches{V_1}{\tnum} \; K_0 == K_1 }{\matches{[ \, \{ K_0 : V_0 \} , \{ K_1 : V_1\} ] \, }{\msf{\tau}}}

%\ir{S-Array-Reccur}{\matches{K_{n-1}}{\tstr} \; \matches{K_n}{\tstr} \; \matches{V_{n-1}}{\tnum} \;  \matches{V_n}{\tnum} \; K_{n-1} == K_n }{\matches{[ \, ... \{ K_{n-1} : V_{n-1} \} , \{ K_n : V_n\} ] \, }{[ \, ... \{ K_{n-2} : V_{n-2} \} , \{ K_{n-1} : V_{n-1}\} ...] \,}}

% Inference rules go here

\end{mathpar}

\problem{Problem 2}

Part 1:

\begin{mathpar}

\ir{Epsilon-Accessor}{\  }{\  ( \, \aeps , j ) \, \mapsto  j \, }

\ir{Key-Accessor}{\ s^{'} \in s }{\  ( \, .s^{'}a, \{(s:j)^{*}\} ) \, \mapsto ( \, a : j_{s^{'}} )\, }

\ir{Array-Accessor}{\ 0 \leq k \leq n}{\ ( \, [\, k]a, \; [ \, j_0, j_1, j_2, ...,j_k,..., j_n]\, )\, \mapsto (\, a, j_k)\,}

\ir{Mpas-Epsilon-Accessor}{\ }{ (\,|\aeps , [ \, j_0, j_1, j_2, ...,j_k,..., j_n]\, ) \mapsto( \aeps , \, [ j_0, j_1, j_2, ...,j_k,..., j_n] )  } \\

\ir{Maps-Accessor}{\ \steps{a}{a^{'}} \,\,\,\, \forall i \in [|j|]. \steps{(a, j_{i})}{(a', j^{'}_{i})} }{( \, |a, [\, j_1, ..., j_k,...,j_n ]\, )\, \mapsto (\,  |a^{'}, [\, j^{'}_1, ..., j^{'}_k,...,j^{'}_n ]\,)\,]\, }
\end{mathpar}

Part 2:

\begin{mathpar}
\ir{Valid-Epsilon-Accessor}{\  }{\ \matches{\aeps}{\tau}}

\ir{Valid-Key-Accessor}{\ \matches{\{(\,s:j)^{*}\,\}}{ \tau} \,\,\, s^{'} \in s \,\,\,\, \matches{j}{\tau^{'}} \,\,\, \matches{a}{\tau^{'}} }{\ \matches{.s^{'}a}{\tau}}

\ir{Valid-Array-Accessor}{ \matches{[\, j ]\,}{\tau} \,\,\, \matches{j}{\tau^{'}} \,\,\,   \matches{a}{\tau^{'}}}{\ \matches{[\, n ]a\,}{\tau}}

\ir{Valid-Maps-Accessor}{ \matches{[\, j ]\,}{\tau} \,\,\,  \matches{j}{\tau^{'}} \,\,\, \matches{a}{\tau^{'}} }{\matches{|a}{\tau}}

%\ir{Valid-Key-Accessor1}{\matches{ \{(\,s:j)\,\}}{\tau} \,\,\, \matches{a}{\tau} \,\,\, \matches{s}{\tstr}  }{\ \matches{.sa}{\tau}}

%\ir{Valid-Array-Accessor1}{\matches{  [\, j ]\,}{\tau} \,\,\, \matches{a}{\tau} \,\,\, n \leq size \, of \, array  }{\ \matches{[\, n ]\,a}{\tau}}

%\ir{Valid-Maps-Accessor1}{\matches{  [\, j ]\,}{\tau} \,\,\, \matches{a}{\tau} }{\matches{|a}{\tau}}

\end{mathpar}

\textit{Accessor safety}: for all $a, j, \tau$, if $\matches{a}{\tau}$ and $\matches{j}{\tau}$, then there exists a $j'$ such that $\evals{(a, j)}{\aeps, j'}$.

\begin{proof}
$P(a) = \forall j, \tau \, . \,\,\, \matches{a}{\tau} \land \matches{j}{\tau} \implies (a, j) \overset{*}{\mapsto} (\aeps, j^{'}) $

Now we want to prove that

$\forall a P(a) \iff P(\aeps) \land (\forall a P(a) \Rightarrow P(.sa)) \land (\forall a P(a) \Rightarrow P([n]a)) \land (\forall a P(a) \Rightarrow P(|a))$

Induction Hypothesis (IH): 
$\forall a P(a) \, holds \, true,\, i.e \,we \,accept\, that\,  (a, j) \overset{*}{\mapsto} (\aeps, j^{'}) \,
where\, \matches{a}{\tau} \land \matches{j}{\tau} $

$\bullet$ Let $a =  \aeps$ then based on EPSILON-ACCESSOR rule defined in problem 2.1 it is trivial to see that accessor safety holds for $\aeps$

$\bullet$ Let P(.sa) if we have $\matches{.sa}{\tau^{'}}$ then by inversion on VALID-KEY-ACCESSOR rule we know that
$\tau^{'} = {(s : \tau)^{}*} \land \matches{a}{\tau}$ 

now for any $\matches{j^{''}}{\tau^{'}}$ based on KEY-ACCESSOR rule defined in problem 2.1 we have
$(.sa, j^{''}) \mapsto (a, j)$ and then due to IH we can have $(a, j) \overset{*}{\mapsto} (\aeps, j^{'})$
thus $(.sa, j^{''}) \overset{*}{\mapsto} (\aeps, j^{'}) $


$\bullet$ Let P([n]a) if we have $\matches{[n]a}{\tau^{'}}$ then by inversion on VALID-ARRAY-ACCESSOR rule we know that
$\tau^{'} = [\tau] \land \matches{a}{\tau}$ 

now for any $\matches{j^{''}}{\tau^{'}}$ based on ARRAY-ACCESSOR rule defined in problem 2.1 we have
$([n]a, j^{''}) \mapsto (a, j)$ and then due to IH we can have $(a, j) \overset{*}{\mapsto} (\aeps, j^{'})$
thus $([n]a, j^{''}) \overset{*}{\mapsto} (\aeps, j^{'}) $

$\bullet$ Let P(|a) if we have $\matches{|a}{\tau^{'}}$ then by inversion on VALID-MAPS-ACCESSOR rule we know that
$\tau^{'} = [\tau] \land \matches{a}{\tau}$ 

now for any $\matches{j^{''}}{\tau^{'}}$ based on MAPS-ACCESSOR rule defined in problem 2.1 we have
$(|a, j^{''}) \mapsto (|a^{'}, j)$ now based on IH we can assume $a^{'}$ is safe accessor on $j$ by using MAPS-ACCESSOR and MAPS-EPSILON-ACCESSOR as required (each time for next accessor IH holds true) and then  we can have $(|a^{'}, j) \overset{*}{\mapsto} (\aeps, j^{'})$
thus $(|a, j^{''}) \overset{*}{\mapsto} (\aeps, j^{'}) $

Thus for all cases accessor safety holds.



%$\bullet$ Induction hypothesis: Let ${A = a_1 a_2 ... a_n}$ is series of accessor  for which $\textbf{\emph{Accessor safety}}$ holds true.


%$(\, A, j)\, \overset{*}{\mapsto} (\, \aeps, j')\,$

%$\bullet$ Let say $(\, .sA, j_0) \mapsto (\, A, j) $ then by inversion lemma of VALID-KEY-ACCESSOR $\matches{j_0}{ \{(\,s:j)\,\}} $ and due to induction hypothesis following holds true
%$(\, .sA, j_0)\, \overset{*}{\mapsto} (\, \aeps, j')\,$ thus accessor safety holds true.

%$\bullet$ Let say $(\, [n]A, j_0) \mapsto (\, A, j) $ then by inversion lemma of VALID-ARRAY-ACCESSOR $\matches{j_0}{ [\, j ]\,} $ and due to induction hypothesis following holds true
%$(\, [n]A, j_0)\, \overset{*}{\mapsto} (\, \aeps, j')\,$ thus accessor safety holds true.

%$\bullet$ Let say $(\, |A, j_0) \mapsto (\, A, j) $ then by inversion lemma of VALID-MAPS-ACCESSOR $\matches{j_0}{ [\, j ]\,} $ and due to induction hypothesis holds true for all values in $[\, j]\, $, \, folloding holds true
%$(\, |A, j_0)\, \overset{*}{\mapsto} (\, \aeps, j')\,$ thus accessor safety holds true.

%Thus with structural induction we have proved that if $\textbf{\emph{Accessor safety}}$ holds on sub-part then it holds for valid composition of accesor sequence.





\end{proof}

\end{document}
